Make pattern translation erase implicit attributes

src/Translation.v
@@ -39,12 +39,12 @@ Section translate_pattern.
     | None => plan
     end.
 
-  Fixpoint translate_pattern (pi : Pattern.t) : ExecutionPlan.t :=
+  Fixpoint translate_pattern' (pi : Pattern.t) : ExecutionPlan.t :=
     match pi with
     | Pattern.start pv => 
         translate_pvertex pv (ScanVertices (vname pv))
     | Pattern.hop pi pe pv =>
-      let plan := translate_pattern pi in
+      let plan := translate_pattern' pi in
       let plan :=
         if (In_decb (vname pv) (dom_vertices pi)) then
           Expand Into (vname (last pi)) (ename pe) (vname pv) (edir pe) plan
@@ -52,6 +52,9 @@ Section translate_pattern.
           Expand All (vname (last pi)) (ename pe) (vname pv) (edir pe) plan
       in translate_pvertex pv (translate_pedge pe plan)
     end.
+
+  Definition translate_pattern (pi : Pattern.t) : ExecutionPlan.t :=
+    ReturnAll (translate_pattern' pi).
 End translate_pattern.
 
 Ltac desf_translate_pvertex_pedge :=
@@ -59,8 +62,8 @@ Ltac desf_translate_pvertex_pedge :=
   desf; simpls;
   normalize_bool.
 
-Theorem type_of__translate_pattern pi (Hwf : Pattern.wf pi) :
-  type_of (translate_pattern pi) = PatternT.type_of Full pi.
+Theorem translate_pattern'_type pi (Hwf : Pattern.wf pi) :
+  type_of (translate_pattern' pi) = PatternT.type_of Full pi.
 Proof.
   all: induction pi; simpls.
   all: desf_translate_pvertex_pedge.
@@ -72,41 +75,49 @@ Proof.
   all: rewrite <- PatternT.In_dom_vertices__iff; auto.
 Qed.
 
-Corollary translate_pattern__type_of_GVertexT pi n (Hwf : Pattern.wf pi) :
-  (In n (Pattern.dom_vertices pi) <-> type_of (translate_pattern pi) n = Some Value.GVertexT).
+Theorem translate_pattern_type pi (Hwf : Pattern.wf pi) :
+  type_of (translate_pattern pi) = PatternT.type_of Explicit pi.
 Proof.
-  rewrite type_of__translate_pattern; auto.
+  unfold translate_pattern. simpls.
+  rewrite translate_pattern'_type; auto.
+  now rewrite PatternT.explicit_projT_type_of.
+Qed.
+
+Corollary translate_pattern'_type_of_GVertexT pi n (Hwf : Pattern.wf pi) :
+  (In n (Pattern.dom_vertices pi) <-> type_of (translate_pattern' pi) n = Some Value.GVertexT).
+Proof.
+  rewrite translate_pattern'_type; auto.
   now rewrite PatternT.In_dom_vertices__iff.
 Qed.
 
-Corollary translate_pattern__type_of_GEdgeT pi n (Hwf : Pattern.wf pi) :
-  (In n (Pattern.dom_edges pi) <-> type_of (translate_pattern pi) n = Some Value.GEdgeT).
+Corollary translate_pattern'_type_of_GEdgeT pi n (Hwf : Pattern.wf pi) :
+  (In n (Pattern.dom_edges pi) <-> type_of (translate_pattern' pi) n = Some Value.GEdgeT).
 Proof. 
-  rewrite type_of__translate_pattern; auto.
+  rewrite translate_pattern'_type; auto.
   now rewrite PatternT.In_dom_edges__iff.
 Qed.
 
-Theorem translate_pattern__type_of__types pi n :
-  type_of (translate_pattern pi) n = Some Value.GVertexT \/
-  type_of (translate_pattern pi) n = Some Value.GEdgeT \/
-  type_of (translate_pattern pi) n = None.
+Theorem translate_pattern'_type_of__types pi n :
+  type_of (translate_pattern' pi) n = Some Value.GVertexT \/
+  type_of (translate_pattern' pi) n = Some Value.GEdgeT \/
+  type_of (translate_pattern' pi) n = None.
 Proof.
   edestruct type_of_types as [H | [H | H]]; eauto.
 Qed.
 
-Corollary translate_pattern__type_of_None pi n (Hwf : Pattern.wf pi)
+Corollary translate_pattern'__type_of_None pi n (Hwf : Pattern.wf pi)
   (HIn_vertices : ~ In n (Pattern.dom_vertices pi))
   (HIn_edges    : ~ In n (Pattern.dom_edges pi)) :
-    type_of (translate_pattern pi) n = None.
+    type_of (translate_pattern' pi) n = None.
 Proof.
-  edestruct translate_pattern__type_of__types as [H | [H | H]]; eauto.
-  1: eapply translate_pattern__type_of_GVertexT in H; try eassumption.
-  2: eapply translate_pattern__type_of_GEdgeT in H; try eassumption.
+  edestruct translate_pattern'_type_of__types as [H | [H | H]]; eauto.
+  1: eapply translate_pattern'_type_of_GVertexT in H; try eassumption.
+  2: eapply translate_pattern'_type_of_GEdgeT in H; try eassumption.
   all: congruence.
 Qed.
 
-Theorem translate_pattern_wf pi (Hwf : Pattern.wf pi) :
-  ExecutionPlan.wf (translate_pattern pi).
+Theorem translate_pattern'_wf pi (Hwf : Pattern.wf pi) :
+  ExecutionPlan.wf (translate_pattern' pi).
 Proof.
   induction pi; simpls.
   2: assert (Pattern.wf pi) by (eapply Pattern.hop_wf; eassumption).
@@ -114,15 +125,22 @@ Proof.
   all: desf; simpls; splits; auto.
   all: normalize_bool.
   all: desf_unfold_pat.
-  all: try apply translate_pattern__type_of_GVertexT; try assumption.
-  all: try apply translate_pattern__type_of_GEdgeT; try assumption.
-  all: try apply translate_pattern__type_of_None; try assumption.
+  all: try apply translate_pattern'_type_of_GVertexT; try assumption.
+  all: try apply translate_pattern'_type_of_GEdgeT; try assumption.
+  all: try apply translate_pattern'__type_of_None; try assumption.
   all: eauto with pattern_wf_db.
 
   all: try contradiction.
   all: try intro; exfalso.
   all: try (eapply Pattern.wf__pv_neq_pe; now eauto).
   all: try (eapply Pattern.wf__last_neq_pe; now eauto).
+Qed.
+
+Theorem translate_pattern_wf pi (Hwf : Pattern.wf pi) :
+  ExecutionPlan.wf (translate_pattern pi).
+Proof.
+  unfold translate_pattern. simpls.
+  now apply translate_pattern'_wf.
 Qed.
 
 Module EvalQueryImpl (S : ExecutionPlan.Spec) : EvalQuery.Spec.
@@ -145,11 +163,11 @@ Module EvalQueryImpl (S : ExecutionPlan.Spec) : EvalQuery.Spec.
   Theorem match_clause_type graph pi table'
     (Hres : eval_match_clause graph pi = Some table')
     (Hwf : Pattern.wf pi) :
-      BindingTable.of_type table' (PatternT.type_of Full pi).
+      BindingTable.of_type table' (PatternT.type_of Explicit pi).
   Proof.
     unfold eval_match_clause in Hres.
     apply eval_type_of in Hres.
-    rewrite type_of__translate_pattern in Hres; auto.
+    now rewrite translate_pattern_type in Hres.
   Qed.
 
   Ltac desf_match_result Hres :=
@@ -157,9 +175,9 @@ Module EvalQueryImpl (S : ExecutionPlan.Spec) : EvalQuery.Spec.
     desf_translate_pvertex_pedge;
     unfold option_bind in *; desf.
 
-  Theorem match_clause_reduce graph pi pe pv table'
-    (Hres : eval_match_clause graph (Pattern.hop pi pe pv) = Some table') :
-      exists table, eval_match_clause graph pi = Some table.
+  Theorem eval_translate_pattern'_reduce graph pi pe pv table'
+    (Hres : eval graph (translate_pattern' (Pattern.hop pi pe pv)) = Some table') :
+      exists table, eval graph (translate_pattern' pi) = Some table.
   Proof.
     desf_match_result Hres.
     all: eauto.
@@ -184,37 +202,6 @@ Module EvalQueryImpl (S : ExecutionPlan.Spec) : EvalQuery.Spec.
     expansion_of graph r' r mode
       (Pattern.vname (Pattern.last pi)) (Pattern.ename pe) (Pattern.vname pv) (Pattern.edir pe).
 
-  Lemma matches_pattern_type_exclude_All pi pe pv r'
-    (Hwf : Pattern.wf (Pattern.hop pi pe pv))
-    (Htype : Rcd.type_of r' = PatternT.type_of Full (Pattern.hop pi pe pv))
-    (HIn : ~ In (Pattern.vname pv) (Pattern.dom_vertices pi)) :
-      Rcd.type_of (Pattern.ename pe !-> None; Pattern.vname pv !-> None; r') =
-        PatternT.type_of Full pi.
-  Proof.
-    assert (Hwf': Pattern.wf pi) by (eauto with pattern_wf_db).
-    repeat rewrite Rcd.type_of_t_update; simpls.
-    rewrite Htype; clear Htype; unfold PartialMap.update.
-    extensionality k.
-    desf_unfold_pat.
-    { erewrite <- PatternT.wf__type_of_pe; eauto. }
-    { erewrite <- PatternT.wf__type_of_pv__None; eauto. }
-  Qed.
-
-  Lemma matches_pattern_type_exclude_Into pi pe pv r'
-    (Hwf : Pattern.wf (Pattern.hop pi pe pv))
-    (Htype : Rcd.type_of r' = PatternT.type_of Full (Pattern.hop pi pe pv))
-    (HIn : In (Pattern.vname pv) (Pattern.dom_vertices pi)) :
-      Rcd.type_of (Pattern.ename pe !-> None; r') = PatternT.type_of Full pi.
-  Proof.
-    assert (Hwf': Pattern.wf pi) by (eauto with pattern_wf_db).
-    rewrite Rcd.type_of_t_update; simpls.
-    rewrite Htype; clear Htype; unfold PartialMap.update.
-    extensionality k.
-    desf_unfold_pat.
-    { erewrite <- PatternT.wf__type_of_pe; eauto. }
-    { erewrite <- PatternT.wf__type_of_pv__Some; eauto. }
-  Qed.
-
   Lemma matches_hop_All graph path e v pi pe pv r'
     (Hwf : Pattern.wf (Pattern.hop pi pe pv))
     (Htype : Rcd.type_of r' = PatternT.type_of Full (Pattern.hop pi pe pv))
@@ -238,7 +225,7 @@ Module EvalQueryImpl (S : ExecutionPlan.Spec) : EvalQuery.Spec.
       exfalso; apply HIn. rewrite e0. apply Pattern.last__dom_vertices. }
     { apply Path.matches_exclude. apply Path.matches_exclude.
       all: eauto with pattern_wf_db. }
-    { apply matches_pattern_type_exclude_All; eauto. }
+    { apply PatternT.matches_pattern_type_exclude_All; eauto. }
   Qed.
 
   Lemma matches_hop_Into graph path e v pi pe pv r'
@@ -266,11 +253,11 @@ Module EvalQueryImpl (S : ExecutionPlan.Spec) : EvalQuery.Spec.
       eauto using Path.matches_full_last. }
     { apply Path.matches_exclude.
       all: eauto with pattern_wf_db. }
-    { eapply matches_pattern_type_exclude_Into; eauto. }
+    { eapply PatternT.matches_pattern_type_exclude_Into; eauto. }
   Qed.
 
-  Theorem match_clause_spec graph path pi table' r'
-    (Hres : eval_match_clause graph pi = Some table')
+  Lemma eval_translate_pattern'_spec graph path pi table' r'
+    (Hres : eval graph (translate_pattern' pi) = Some table')
     (Hwf : Pattern.wf pi)
     (Htype : Rcd.type_of r' = PatternT.type_of Full pi)
     (Hmatch : Path.matches Full graph r' path pi) :
@@ -312,6 +299,20 @@ Module EvalQueryImpl (S : ExecutionPlan.Spec) : EvalQuery.Spec.
     all: eauto with pattern_wf_db.
   Qed.
 
+  Theorem match_clause_spec graph path pi table' r'
+    (Hres : eval_match_clause graph pi = Some table')
+    (Hwf : Pattern.wf pi)
+    (Htype : Rcd.type_of r' = PatternT.type_of Explicit pi)
+    (Hmatch : Path.matches Explicit graph r' path pi) :
+      In r' table'.
+  Proof.
+    desf_match_result Hres.
+    eapply Path.matches_explicit_exists_proj in Hmatch; auto.
+    desf.
+    eapply return_all_spec; eauto.
+    eapply eval_translate_pattern'_spec; eauto.
+  Qed.
+
   Lemma matches_expansion_of graph mode r r' path v_from e v_to pi pe pv
     (Hg_wf : PropertyGraph.wf graph)
     (Hwf : Pattern.wf (Pattern.hop pi pe pv))
@@ -327,8 +328,7 @@ Module EvalQueryImpl (S : ExecutionPlan.Spec) : EvalQuery.Spec.
     all: try apply Path.matches_exclude.
     all: try apply Path.matches_exclude.
     all: eauto using Path.matches_full_in_dom_contra.
-    all: try apply Path.Build_matches_pedge.
-    all: try apply Path.Build_matches_pvertex.
+    all: try constructor.
     all: autounfold with matches_name_db in *.
     all: auto.
 
@@ -345,8 +345,8 @@ Module EvalQueryImpl (S : ExecutionPlan.Spec) : EvalQuery.Spec.
     all: edestruct ends_In; eauto.
   Qed.
 
-  Theorem match_clause_spec' graph pi table' r'
-    (Hres : eval_match_clause graph pi = Some table')
+  Lemma eval_translate_pattern'_spec' graph pi table' r'
+    (Hres : eval graph (translate_pattern' pi) = Some table')
     (Hg_wf : PropertyGraph.wf graph)
     (Hwf : Pattern.wf pi)
     (HIn : In r' table') :
@@ -386,5 +386,19 @@ Module EvalQueryImpl (S : ExecutionPlan.Spec) : EvalQuery.Spec.
     all: ins.
     all: try unfold expansion_of' in *; desf.
     all: desf_unfold_pat.
+  Qed.
+
+  Theorem match_clause_spec' graph pi table' r'
+    (Hres : eval_match_clause graph pi = Some table')
+    (Hg_wf : PropertyGraph.wf graph)
+    (Hwf : Pattern.wf pi)
+    (HIn : In r' table') :
+      exists path, Path.matches Explicit graph r' path pi.
+  Proof.
+    desf_match_result Hres.
+    eapply return_all_spec' in HIn; eauto; desf.
+    edestruct eval_translate_pattern'_spec'; eauto.
+    eexists.
+    eapply Path.matches_explicit_proj; eauto.
   Qed.
 End EvalQueryImpl.
