src/Semantics.v
@@ -4,6 +4,7 @@ Require Import Bool.
 Require Import BinNums.
 From Coq Require Import Classes.EquivDec.
 From Coq Require Import Logic.FunctionalExtensionality.
+From Coq Require Import Lia.
 Import ListNotations.
 
 From hahn Require Import HahnBase.
@@ -78,6 +79,21 @@ Module PatternT.
     eauto with pattern_wf_db.
   Qed.
 
+  Lemma type_of_explicit__dom_vertices (pi : Pattern.t) nv
+    (Hwf : Pattern.wf pi)
+    (HIn : In (Name.explicit nv) (Pattern.dom_vertices pi)) :
+      type_of Explicit pi (Name.explicit nv) = Some Value.GVertexT.
+  Proof.
+    induction pi; simpls.
+    all: desf; simpls; desf.
+    all: try apply PartialMap.update_eq.
+
+    all: desf_unfold_pat.
+    all: eauto with pattern_wf_db.
+    all: exfalso; eapply Pattern.wf__pe__dom_vertices; eauto.
+    all: now rewrite Heq0, e.
+  Qed.
+
   Lemma type_of__dom_edges (pi : Pattern.t) ne
     (Hwf : Pattern.wf pi)
     (HIn : In ne (Pattern.dom_edges pi)) :
@@ -95,22 +111,43 @@ Module PatternT.
     { eapply Pattern.wf__pv__dom_edges; eauto. }
   Qed.
 
-  Lemma dom_vertices__type_of (pi : Pattern.t) nv
+  Lemma type_of_explicit__dom_edges (pi : Pattern.t) ne
     (Hwf : Pattern.wf pi)
-    (Htype : type_of Full pi nv = Some Value.GVertexT) :
-      In nv (Pattern.dom_vertices pi).
+    (HIn : In (Name.explicit ne) (Pattern.dom_edges pi)) :
+      type_of Explicit pi (Name.explicit ne) = Some Value.GEdgeT.
   Proof.
     induction pi; simpls.
+    all: desf.
+    all: try apply PartialMap.update_eq.
+    all: try rewrite PartialMap.update_neq.
+    all: try apply PartialMap.update_eq.
+    all: try rewrite PartialMap.update_neq.
+    all: eauto with pattern_wf_db.
+    
+    all: intro; subst.
+    { eapply Pattern.wf__pv_neq_pe; eauto. now rewrite Heq, H, Heq0. }
+    { eapply Pattern.wf__pe__dom_edges; eauto. now rewrite Heq0, H. }
+    { eapply Pattern.wf__pv__dom_edges; eauto. now rewrite Heq, H. }
+    { eapply Pattern.wf__pv__dom_edges; eauto. now rewrite Heq, H. }
+    { eapply Pattern.wf__pe__dom_edges; eauto. now rewrite Heq0, H. }
+  Qed.
+
+  Lemma dom_vertices__type_of mode pi nv
+    (Hwf : Pattern.wf pi)
+    (Htype : type_of mode pi nv = Some Value.GVertexT) :
+      In nv (Pattern.dom_vertices pi).
+  Proof.
+    induction pi, mode; simpls.
     all: desf_unfold_pat.
     all: eauto with pattern_wf_db.
   Qed.
 
-  Lemma dom_edges__type_of (pi : Pattern.t) ne
+  Lemma dom_edges__type_of mode pi ne
     (Hwf : Pattern.wf pi)
-    (Htype : type_of Full pi ne = Some Value.GEdgeT) :
+    (Htype : type_of mode pi ne = Some Value.GEdgeT) :
       In ne (Pattern.dom_edges pi).
   Proof.
-    induction pi; simpls.
+    induction pi, mode; simpls.
     all: desf_unfold_pat.
     all: eauto with pattern_wf_db.
   Qed.
@@ -127,6 +164,32 @@ Module PatternT.
       In ne (Pattern.dom_edges pi) <-> type_of Full pi ne = Some Value.GEdgeT.
   Proof.
     split; eauto using type_of__dom_edges, dom_edges__type_of.
+  Qed.
+
+  Theorem In_dom_vertices_explicit__iff (pi : Pattern.t) nv
+    (Hwf : Pattern.wf pi) :
+      In (Name.explicit nv) (Pattern.dom_vertices pi) <->
+        type_of Explicit pi (Name.explicit nv) = Some Value.GVertexT.
+  Proof.
+    split; eauto using type_of_explicit__dom_vertices, dom_vertices__type_of.
+  Qed.
+
+  Theorem In_dom_edges_explicit__iff (pi : Pattern.t) ne
+    (Hwf : Pattern.wf pi) :
+      In (Name.explicit ne) (Pattern.dom_edges pi) <->
+        type_of Explicit pi (Name.explicit ne) = Some Value.GEdgeT.
+  Proof.
+    split; eauto using type_of_explicit__dom_edges, dom_edges__type_of.
+  Qed.
+
+  Theorem type_of_explicit__implicit (pi : Pattern.t) n :
+    type_of Explicit pi (Name.implicit n) = None.
+  Proof.
+    induction pi; simpls.
+    all: desf; simpls; desf.
+    all: repeat rewrite PartialMap.update_neq.
+    all: auto.
+    all: ins; discriminate.
   Qed.
 
   Theorem type_of__types mode pi k :
@@ -153,7 +216,34 @@ Module PatternT.
     congruence.
   Qed.
 
-  Corollary not_In_dom__iff (pi : Pattern.t) k
+  Theorem In_dom mode pi k
+    (Hwf : Pattern.wf pi)
+    (Hdom : PartialMap.in_dom k (type_of mode pi)) :
+      In k (Pattern.dom pi).
+  Proof.
+    unfold PartialMap.in_dom in *.
+    destruct Hdom as [v Htype].
+    rewrite Pattern.In_dom.
+    destruct mode eqn:Heq, k.
+    all: try (rewrite type_of_explicit__implicit in Htype; discriminate).
+    1: rewrite In_dom_vertices_explicit__iff, In_dom_edges_explicit__iff; auto.
+    all: try rewrite In_dom_vertices__iff, In_dom_edges__iff; auto.
+    all: edestruct type_of__types with (mode := mode) (pi := pi) as [? | [? | ?]].
+    all: desf.
+    all: simpls; eauto.
+    all: congruence.
+  Qed.
+
+  Theorem not_In_dom mode pi k
+    (Hwf : Pattern.wf pi)
+    (HIn : ~ (In k (Pattern.dom pi))) :
+      type_of mode pi k = None.
+  Proof.
+    rewrite <- PartialMap.not_in_dom_iff.
+    ins; eauto using In_dom.
+  Qed.
+
+  Theorem not_In_dom__iff (pi : Pattern.t) k
     (Hwf : Pattern.wf pi) :
       ~ (In k (Pattern.dom pi)) <-> type_of Full pi k = None.
   Proof.
@@ -161,35 +251,86 @@ Module PatternT.
     now rewrite PartialMap.not_in_dom_iff.
   Qed.
 
-  Lemma wf__type_of_pe pi pe pv
+  Lemma wf__type_of_pe mode pi pe pv
     (Hwf : Pattern.wf (Pattern.hop pi pe pv)) :
-      type_of Full pi (Pattern.ename pe) = None.
+      type_of mode pi (Pattern.ename pe) = None.
   Proof.
-    rewrite <- not_In_dom__iff. 
+    apply not_In_dom.
     all: eauto with pattern_wf_db.
   Qed.
 
-  Lemma wf__type_of_pv__None pi pe pv
+  Lemma wf__type_of_pv__None mode pi pe pv
     (Hwf : Pattern.wf (Pattern.hop pi pe pv))
     (HIn : ~ In (Pattern.vname pv) (Pattern.dom_vertices pi)) :
-      type_of Full pi (Pattern.vname pv) = None.
+      type_of mode pi (Pattern.vname pv) = None.
   Proof.
-    rewrite <- not_In_dom__iff. 
+    apply not_In_dom.
     all: eauto with pattern_wf_db.
   Qed.
 
-  Lemma wf__type_of_pv__Some pi pe pv
+  Lemma wf__type_of_pv__Some mode pi pe pv
     (Hwf : Pattern.wf (Pattern.hop pi pe pv))
     (HIn : In (Pattern.vname pv) (Pattern.dom_vertices pi)) :
-      type_of Full pi (Pattern.vname pv) = Some Value.GVertexT.
+      type_of mode pi (Pattern.vname pv) = Some Value.GVertexT.
   Proof.
-    rewrite <- In_dom_vertices__iff. 
-    all: eauto with pattern_wf_db.
+    assert (Hwf': Pattern.wf pi) by (eauto with pattern_wf_db).
+    destruct mode, (Pattern.vname pv) eqn:Heq.
+    all: try (exfalso; eapply Pattern.wf__imp_pv__dom_vertices; now eauto).
+    { now rewrite <- In_dom_vertices_explicit__iff. }
+    { now rewrite <- In_dom_vertices__iff. }
   Qed.
 
   #[global]
   Hint Resolve wf__type_of_pe wf__type_of_pv__None wf__type_of_pv__Some : patternT_wf_db.
 
+  Lemma explicit_projT_type_of mode pi :
+    Rcd.explicit_projT (type_of mode pi) = type_of Explicit pi.
+  Proof.
+    destruct mode.
+    all: induction pi; simpls.
+    all: unfold Rcd.explicit_projT in *.
+    all: extensionality k.
+    all: try apply (f_equal (fun f => f k)) in IHpi.
+    all: desf_unfold_pat.
+  Qed.
+
+  Theorem matches_pattern_type_exclude_All mode pi pe pv r'
+    (Hwf : Pattern.wf (Pattern.hop pi pe pv))
+    (Htype : Rcd.type_of r' = PatternT.type_of mode (Pattern.hop pi pe pv))
+    (HIn : ~ In (Pattern.vname pv) (Pattern.dom_vertices pi)) :
+      Rcd.type_of (Pattern.ename pe !-> None; Pattern.vname pv !-> None; r') =
+        PatternT.type_of mode pi.
+  Proof.
+    assert (Hwf': Pattern.wf pi) by (eauto with pattern_wf_db).
+    repeat rewrite Rcd.type_of_t_update; simpls.
+    rewrite Htype; clear Htype; unfold PartialMap.update.
+    destruct mode; simpls.
+    all: extensionality k.
+    all: desf_unfold_pat.
+    { erewrite PatternT.wf__type_of_pe with (mode := Explicit); eauto. }
+    { erewrite PatternT.wf__type_of_pv__None with (mode := Explicit); eauto. }
+    { erewrite PatternT.wf__type_of_pe with (mode := Full); eauto. }
+    { erewrite PatternT.wf__type_of_pv__None with (mode := Full); eauto. }
+  Qed.
+
+  Lemma matches_pattern_type_exclude_Into mode pi pe pv r'
+    (Hwf : Pattern.wf (Pattern.hop pi pe pv))
+    (Htype : Rcd.type_of r' = PatternT.type_of mode (Pattern.hop pi pe pv))
+    (HIn : In (Pattern.vname pv) (Pattern.dom_vertices pi)) :
+      Rcd.type_of (Pattern.ename pe !-> None; r') = PatternT.type_of mode pi.
+  Proof.
+    assert (Hwf': Pattern.wf pi) by (eauto with pattern_wf_db).
+    rewrite Rcd.type_of_t_update; simpls.
+    rewrite Htype; clear Htype; unfold PartialMap.update.
+    destruct mode; simpls.
+    all: extensionality k.
+    all: desf_unfold_pat.
+    { erewrite PatternT.wf__type_of_pe with (mode := Explicit); eauto. }
+    1-2: rewrite <- Heq0 in *.
+    1-2: now (erewrite PatternT.wf__type_of_pv__Some with (mode := Explicit); eauto).
+    { erewrite PatternT.wf__type_of_pe with (mode := Full); eauto. }
+    { erewrite PatternT.wf__type_of_pv__Some with (mode := Full); eauto. }
+  Qed.
 End PatternT.
 
 Module Path.
@@ -392,18 +533,134 @@ Module Path.
     destruct mode.
     all: induction Hmatch.
     all: destruct Hpv; try destruct Hpe.
-    all: try apply matches_nil.
-    all: try apply matches_cons.
-    all: unfold matches_name in *; desf.
+    all: constructor; auto.
     all: try apply IHHmatch.
     all: try (intro; apply HIn; right; now right).
-    all: try apply Path.Build_matches_pvertex.
-    all: try apply Path.Build_matches_pedge.
-    all: auto.
+    all: constructor; auto.
     all: autounfold with matches_name_db in *.
     all: desf; ins.
     all: desf_unfold_pat.
     all: exfalso; auto.
+  Qed.
+
+  Theorem matches_explicit_proj mode graph path pi r
+    (Hmatch : matches mode graph r path pi) :
+      matches Explicit graph (Rcd.explicit_proj r) path pi.
+  Proof.
+    destruct mode.
+    all: induction Hmatch.
+    all: destruct Hpv; try destruct Hpe.
+    all: constructor; auto.
+    all: constructor; auto.
+    all: autounfold with matches_name_db in *.
+    all: desf.
+  Qed.
+
+  Theorem matches_explicit mode graph path pi r
+    (Hmatch : matches mode graph r path pi) :
+      matches Explicit graph r path pi.
+  Proof.
+    destruct mode.
+    { assumption. }
+    induction Hmatch.
+    all: destruct Hpv; try destruct Hpe.
+    all: constructor; auto.
+    all: constructor; auto.
+    all: autounfold with matches_name_db in *.
+    all: desf.
+  Qed.
+
+  Theorem matches_two_records graph path pi r1 r2 n
+    (Hmatch1 : matches Explicit graph r1 path pi)
+    (Hmatch2 : matches Explicit graph r2 path pi)
+    (HIn1 : In (Name.explicit n) (Pattern.dom pi)) :
+      r1 (Name.explicit n) = r2 (Name.explicit n).
+  Proof.
+    induction Hmatch1; inv Hmatch2.
+    all: destruct Hpv; try destruct Hpe.
+    all: destruct Hpv0; try destruct Hpe0.
+    all: autounfold with matches_name_db in *.
+    all: simpls; desf; auto.
+    all: try now rewrite matches_vname0, matches_vname1.
+    all: try now rewrite matches_ename0, matches_ename1.
+  Qed.
+
+  Theorem matches_explicit_exists_proj graph path pi r'
+    (Hwf : Pattern.wf pi)
+    (Hmatch : matches Explicit graph r' path pi)
+    (Htype  : Rcd.type_of r' = PatternT.type_of Explicit pi) :
+      exists r,
+        << Hproj : r' = Rcd.explicit_proj r >> /\
+        << Hmatch' : matches Full graph r path pi >> /\
+        << Htype' : Rcd.type_of r = PatternT.type_of Full pi >>.
+  Proof.
+    gen_dep path r'.
+    induction pi; intros; inv Hmatch; clear Hmatch.
+    { simpls.
+      exists (Pattern.vname pv |-> Value.GVertex v).
+      all: splits.
+      all: try constructor; try constructor.
+
+      all: destruct Hpv; try destruct Hpe.
+      all: autounfold with matches_name_db in *.
+      all: desf.
+
+      all: try apply PartialMap.update_eq.
+      all: try apply Rcd.type_of_singleton.
+
+      all: extensionality k.
+      all: apply (f_equal (fun f => f k)) in Htype.
+      all: unfold Rcd.type_of, option_map in Htype.
+      all: unfold Rcd.explicit_proj.
+      all: desf_unfold_pat; desf.
+    }
+
+    assert (Hwf': Pattern.wf pi) by (eauto with pattern_wf_db).
+    destruct (In_decbP (Pattern.vname pv) (Pattern.dom_vertices pi)).
+    1: set (r'0 := (Pattern.ename pe !-> None; r')).
+    2: set (r'0 := (Pattern.ename pe !-> None; Pattern.vname pv !-> None; r')).
+    all: specialize IHpi with (r' := r'0); subst r'0.
+    all: edestruct IHpi as [r ?]; eauto; clear IHpi; desf.
+    all: try erewrite PatternT.matches_pattern_type_exclude_All.
+    all: try erewrite PatternT.matches_pattern_type_exclude_Into.
+    all: repeat apply matches_exclude.
+    all: eauto with pattern_wf_db.
+
+    1: exists (Pattern.ename pe |-> Value.GEdge e; r).
+    2: exists (Pattern.vname pv |-> Value.GVertex v;
+               Pattern.ename pe |-> Value.GEdge e; r).
+    all: splits.
+    all: try constructor; try constructor.
+
+    all: destruct Hpv, Hpe.
+    all: repeat apply matches_exclude.
+    all: eauto with pattern_wf_db.
+
+    all: autounfold with matches_name_db in *.
+    all: try apply PartialMap.update_eq.
+    all: try rewrite PartialMap.update_neq.
+    all: try rewrite PartialMap.update_eq.
+
+    all: try (eapply Pattern.wf__pe_neq_pv; now eauto).
+    all: try (eapply Pattern.wf__pv_neq_pe; now eauto).
+    
+    all: repeat rewrite Rcd.type_of_update.
+    all: try rewrite Htype'; clear Htype'.
+    all: try extensionality k.
+    all: try apply (f_equal (fun f => f k)) in Htype.
+    all: try apply (f_equal (fun f => f k)) in Hproj.
+    all: unfold Rcd.type_of, option_map in Htype.
+    all: unfold Rcd.explicit_proj in *; simpls.
+    all: desf_unfold_pat; desf.
+
+    all: try (exfalso; eapply Pattern.wf__imp_pv__dom_vertices; now eauto).
+    all: try (rewrite PatternT.type_of_explicit__implicit in Htype; discriminate).
+
+    all: try (erewrite <- PatternT.In_dom_vertices__iff; auto).
+    
+    all: erewrite matches_two_records; eauto.
+    all: try eapply matches_explicit; eauto.
+    all: rewrite Pattern.In_dom; auto.
   Qed.
 End Path.
 
@@ -640,16 +897,16 @@ Module EvalQuery.
     Axiom match_clause_type : forall graph pattern table',
       eval_match_clause graph pattern = Some table' ->
         Pattern.wf pattern ->
-          BindingTable.of_type table' (PatternT.type_of Full pattern).
+          BindingTable.of_type table' (PatternT.type_of Explicit pattern).
 
     Axiom match_clause_spec : forall graph path pattern table' r',
       eval_match_clause graph pattern = Some table' ->
-        Pattern.wf pattern -> Rcd.type_of r' = PatternT.type_of Full pattern ->
-          Path.matches Full graph r' path pattern -> In r' table'.
+        Pattern.wf pattern -> Rcd.type_of r' = PatternT.type_of Explicit pattern ->
+          Path.matches Explicit graph r' path pattern -> In r' table'.
 
     Axiom match_clause_spec' : forall graph pattern table' r',
       eval_match_clause graph pattern = Some table' ->
         PropertyGraph.wf graph -> Pattern.wf pattern -> In r' table' ->
-          exists path, Path.matches Full graph r' path pattern.
+          exists path, Path.matches Explicit graph r' path pattern.
   End Spec.
 End EvalQuery.
